Make prototype of completeness theorem
 周りでバグがありそうなので  にくるむ？

Kernel.thy
@@ -2,38 +2,65 @@ theory Kernel
   imports Main
 begin
 
-type_synonym name = "nat"
 type_synonym ty_name = "char list"
 
 datatype type =
   Ty_Var ty_name ("_:*" [1000] 999) |
   Fun type type (infixr "\<rightarrow>>" 100)
 
+type_synonym name = "nat"
+(*printable version*)
+(*
+datatype name = X | Y | Z | W
+fun "next" :: "name \<Rightarrow> name" where
+  "next X = Y" |
+  "next Y = Z" |
+  "next Z = W" |
+  "next W = X"
+lemma UNIV_name:
+  "UNIV = {X, Y, Z, W}"
+  by (auto intro: name.exhaust)
+instantiation name :: enum
+begin
+definition
+  "enum_name = [X, Y, Z, W]"
+definition
+  "enum_all_name P \<longleftrightarrow> P X \<and> P Y \<and> P Z \<and> P W"
+definition
+  "enum_ex_name P \<longleftrightarrow> P X \<or> P Y \<or> P Z \<or> P W"
+instance by (intro_classes, auto simp add: enum_name_def enum_all_name_def enum_ex_name_def UNIV_name)
+end
+*)
+
+(*test*)
+\<comment> \<open>
 term "''a'':*"
 term "''a'':* \<rightarrow>> ''b'':*"
+\<close>
 
 datatype "term" =
   Var name type ("_::_" 500) |
   Abs name type "term" ("\<lambda>_:: _. _>" [1000, 998, 499] 999) |
   App "term" "term" ("|[_ _]|")
+
+(*test*)
+\<comment> \<open>
 term "0::''a'':*"
 term "\<lambda>0:: ''a'':*. 0::''a'':*>"
 term "|[\<lambda>0:: ''a'':*. 0::''a'':*> 0::''a'':*]|"
-(*
-(*free variable*)
-fun fv :: "term \<Rightarrow> name set" where
-  "fv (Var n T) = {n}" |
-  "fv (Abs n T t) = fv t - {n}" |
-  "fv (App t1 t2) = fv t1 \<union> fv t2"
-*)
+\<close>
+
 fun type_of :: "term \<Rightarrow> type" where
   "type_of (Var n t) = t" |
   "type_of (Abs n T t) = Fun T (type_of t)" |
   "type_of (App t1 t2) = (case type_of t1 of
     Fun T1 T2 \<Rightarrow> if T1 = type_of t2 then T2 else undefined)"
-(*
-lemma "type_of (App (Var 0 (Ty_Var ''a'')) (Var 1 (Ty_Var ''b''))) = undefined" by simp
-*)
+
+(*test*)
+\<comment> \<open>
+lemma "type_of |[0::''a'':* 1::''b'':*]| = undefined" by simp
+\<close>
+
 type_synonym env = "name \<rightharpoonup> type"
 
 fun env_of :: "term \<Rightarrow> env" where
@@ -41,11 +68,11 @@ fun env_of :: "term \<Rightarrow> env" where
   "env_of (Abs n T t) = (env_of t)(n := None)" |
   "env_of (App t1 t2) = env_of t1 ++ env_of t2"
 
-fun well_typed where
+fun well_typed :: "term \<Rightarrow> bool" where
   "well_typed (Var n T) = True" |
   "well_typed (Abs n T t) = (
     let n_Ty = env_of t n in
-    if n_Ty \<in> {None, Some T} then well_typed t else False)" |
+    if n_Ty = None \<or> n_Ty = Some T then well_typed t else False)" |
   "well_typed (App t1 t2) = (case type_of t1 of
     Fun T _ \<Rightarrow>
       let e1 = env_of t1 in
@@ -54,8 +81,10 @@ fun well_typed where
         well_typed t1 \<and> well_typed t2 |
     _ \<Rightarrow> False)"
 
-lemma "\<not> well_typed (App (0::''a'':*) (1::''b'':*))"
-  by simp
+(*test*)
+\<comment> \<open>
+lemma "\<not> well_typed |[0::''a'':* 1::''b'':*]|" by simp
+\<close>
 
 definition mk_var :: "name \<Rightarrow> type \<Rightarrow> term" where
   "mk_var n T = Var n T"
@@ -68,30 +97,98 @@ definition mk_app :: "term \<Rightarrow> term \<Rightarrow> term" where
     let ret = (App t1 t2) in
     if well_typed ret then ret else undefined)"
 
+(*user accessible function*)
 definition imp_i :: "name \<Rightarrow> type \<Rightarrow> term \<Rightarrow> term" where
   "imp_i = mk_abs"
 definition imp_e :: "term \<Rightarrow> term \<Rightarrow> term" where
   "imp_e = mk_app"
 definition "assume" :: "name \<Rightarrow> type \<Rightarrow> term" where
   "assume = mk_var"
-find_theorems undefined
+
 inductive pr_term where
   "pr_term (assume n T)" |
   "pr_term t \<Longrightarrow> pr_term (imp_i n T t)" |
   "pr_term t1 \<Longrightarrow> pr_term t2 \<Longrightarrow> pr_term (imp_e t1 t2)"
 
+lemma "\<not> well_typed undefined"
+(*lemma "pr_term undefined" sledgehammer*)
+lemma "\<not> pr_term undefined"
+
 lemmas mk_def = mk_var_def mk_abs_def mk_app_def
 lemmas rule_def = imp_i_def imp_e_def assume_def
 
-lemma "pr_term t \<Longrightarrow> t \<noteq> undefined \<Longrightarrow> well_typed t"
-  by (induct rule: pr_term.induct, auto simp add: mk_def rule_def Let_def)
-(*
-lemma "impI ''x'' (Ty_Var ''a'') (assume ''x'' (Ty_Var ''a'')) = (Abs ''x'' (Ty_Var ''a'') (Var ''x'' (Ty_Var ''a'')))"
+(*test*)
+\<comment> \<open>
+lemma "imp_i 0 (''a'':*) (assume 0 (''a'':*)) = (\<lambda>0::''a'':*. 0::''a'':*>)"
   by (simp add: mk_def rule_def)
-lemma "impI ''x'' ()"
-lemma "impI 0 (Ty_Var 1) ()"
-lemma "type_of (impI 0 (Ty_Var 2) (impI 1 (Fun (Ty_Var 2) (Ty_Var 3)) (impE (assume 1 (Fun (Ty_Var 2) (Ty_Var 3))) (assume 0 (Ty_Var 2)))))
- = Fun (Ty_Var 2) (Fun (Fun (Ty_Var 2) Ty_Var 3) (Ty_Var 3))"
-*)
+lemma "type_of (imp_i 0 (''a'':*) (imp_i 1 (''a'':* \<rightarrow>> ''b'':*) (imp_e (assume 1 (''a'':* \<rightarrow>> ''b'':*)) (assume 0 (''a'':*)))))
+  = ''a'':* \<rightarrow>> (''a'':* \<rightarrow>> ''b'':*) \<rightarrow>> ''b'':*"
+  by (simp add: mk_def rule_def)
+\<close>
+
+definition print :: "term \<Rightarrow> type \<times> term" where
+  "print t = (type_of t, t)"
+
+(*test*)
+\<comment> \<open>
+value "print (imp_i X (''a'':*) (assume X (''a'':*)))"
+\<close>
+\<comment> \<open>
+value "print (
+imp_i X (''a'':* \<rightarrow>> ''b'':* \<rightarrow>> ''c'':*) (
+  imp_i Y (''a'':* \<rightarrow>> ''b'':*) (
+    imp_i Z (''a'':*) (
+      imp_e
+        (imp_e
+          (assume X (''a'':* \<rightarrow>> ''b'':* \<rightarrow>> ''c'':*))
+          (assume Z (''a'':*)))
+        (imp_e
+          (assume Y (''a'':* \<rightarrow>> ''b'':*))
+          (assume Z (''a'':*)))
+))))"
+\<close>
+
+theorem soundness: "pr_term t \<Longrightarrow> t \<noteq> undefined \<Longrightarrow> well_typed t"
+  by (induct rule: pr_term.induct, auto simp add: mk_def rule_def Let_def)
+(*lemma "\<exists>t'. pr_term t' \<and> type_of t' = type_of t \<and> t' \<noteq> undefined"
+  apply (cases t)
+    apply (metis mk_def rule_def type_of.simps pr_term.simps)
+   apply (metis mk_def rule_def type_of.simps pr_term.simps)
+  apply (metis mk_def rule_def type_of.simps pr_term.simps)
+  done*)
+lemma "(a::T:*) \<noteq> undefined"
+theorem completeness: "well_typed t \<Longrightarrow> \<exists>t'. pr_term t' \<and> type_of t' = type_of t \<and> t' \<noteq> undefined"
+proof (induct t rule: well_typed.induct)
+  case (1 n T)
+  show ?case
+    apply (rule exI[of _ "assume n T"])
+    apply (subst pr_term.simps)
+    apply auto
+     apply (simp add: rule_def mk_def)
+    find_theorems undefined
+    thm pr_term.simps
+next
+  case (2 n T t)
+  obtain t' where "pr_term t' \<and> type_of t' = type_of t"
+  proof -
+    have "well_typed t"
+      using "2.prems"
+      by (meson well_typed.simps(2))
+    show ?thesis
+      using "2.hyps"[of "Some T"]
+      sorry
+  qed
+  show ?case
+    apply (metis mk_def(1) rule_def(3) pr_term.simps type_of.simps)
+    apply (rule exI[of _ "imp_i n T t"])
+    apply auto
+     apply (rule)
+    using 2
+    apply
+    sorry
+next
+  case (3 t1 t2)
+  then show ?case sorry
+qed
 
 end
